src/tls/Parse.fst
@@ -47,7 +47,7 @@ let tls_region : tls_rgn = new_colored_region HH.root tls_color
 let tls_tables_region : (r:tls_rgn{HH.parent r = tls_region}) =
     new_region tls_region
 
-
+    
 (** End Module Regions *)
 
 
